Add CBT methods specs (no implementations / proofs)

LiveVerif/src/LiveVerifExamples/critbit.v
@@ -4,6 +4,7 @@ Require Import LiveVerifExamples.onesize_malloc.
 Require Import coqutil.Datatypes.PropSet.
 
 (* NOTE THAT THIS FILE STILL ALSO CONTAINS MANY THINGS RELATED TO BSTs *)
+(* some parts of this file are based on tree_set.v (binary search trees) *)
 
 Inductive tree_skeleton: Set :=
 | Leaf
@@ -67,23 +68,27 @@ Definition append_1 (p: prefix) :=
   {| length := p.(length) + 1;
      bits := word.or (canonic_bits p) (bit_at p.(length)) |}.
 
-Fixpoint cbt (sk: tree_skeleton) (p: prefix) (c: word_map) (a: word) : mem -> Prop :=
+Definition full_prefix (k: word) := {| length := 32; bits := k |}.
+
+Fixpoint cbt' (sk: tree_skeleton) (p: prefix) (c: word_map) (a: word): mem -> Prop :=
   match sk with
     | Leaf => ex1 (fun k: word => ex1 (fun v: word =>
-        <{ * emp (c = map.singleton k v)
-           * emp (p.(bits) = k)
-           * emp (p.(length) = 32)
-           * <{ + uintptr k
+        <{ * emp (a <> /[0])
+           * emp (c = map.singleton k v)
+           * emp (p = full_prefix k)
+           * <{ + uint 32 (-1)
+                + uintptr k
                 + uintptr v }> a }>))
   | Node skL skR => ex1 (fun aL: word => ex1 (fun pL: prefix => ex1 (fun cL: word_map =>
      ex1 (fun ix: Z => ex1 (fun aR: word => ex1 (fun pR: prefix => ex1 (fun cR: word_map
           =>
           <{ * emp (a <> /[0])
-             * <{ + uintptr aL
-                  + uint 32 p.(length)
+             * freeable 12 a
+             * <{ + uint 32 p.(length)
+                  + uintptr aL
                   + uintptr aR }> a
-             * cbt skL pL cL aL
-             * cbt skR pR cR aR
+             * cbt' skL pL cL aL
+             * cbt' skR pR cR aR
              * emp (0 <= p.(length) <= 31)
              * emp (is_canonic p)
              * emp (is_prefix (append_0 p) pL)
@@ -91,314 +96,116 @@ Fixpoint cbt (sk: tree_skeleton) (p: prefix) (c: word_map) (a: word) : mem -> Pr
              * emp (map.split c cL cR) }>)))))))
   end.
 
-(*
+Definition nncbt (c: word_map) (a: word): mem -> Prop :=
+  ex1 (fun sk: tree_skeleton => ex1 (fun p: prefix => cbt' sk p c a)).
 
-Fixpoint bst'(sk: tree_skeleton)(s: set Z)(addr: word){struct sk}: mem -> Prop :=
-  match sk with
-  | Leaf => emp (addr = /[0] /\ forall x, ~ s x)
-  | Node skL skR => ex1 (fun p: word => (ex1 (fun v: Z => (ex1 (fun q: word =>
-      <{ * emp (addr <> /[0])
-         * emp (s v)
-         * freeable 12 addr
-         * <{ + uintptr p
-              + uint 32 v
-              + uintptr q }> addr
-         * bst' skL (fun x => s x /\ x < v) p
-         * bst' skR (fun x => s x /\ v < x) q }>)))))
-  end.
+(* in full generality, a CBT can be represented as a pointer which is either
+   - NULL for an empty CBT, or
+   - pointing to the CBT root node *)
+Definition cbt (c: word_map) (a: word): mem -> Prop :=
+  or1 (nncbt c a) (emp (c = map.empty /\ a = /[0])).
 
-(* Note: one level of indirection because sometimes we have to change the root
-   pointer (eg from null (empty) to non-null) or it is convenient *)
-Definition bst(s: set Z)(addr: word): mem -> Prop :=
-  ex1 (fun rootp => <{ * uintptr rootp addr
-                       * freeable 4 addr
-                       * ex1 (fun sk: tree_skeleton => bst' sk s rootp) }>).
+#[export] Instance spec_of_cbt_init: fnspec :=                              .**/
 
-Local Hint Extern 1 (PredicateSize (bst' ?sk)) =>
-  let r := eval cbv iota in
-    (match sk with
-     | Node _ _ => 12
-     | Leaf => 0
-     end) in
-  exact r
-: typeclass_instances.
+uintptr_t cbt_init( ) /**#
+  ghost_args := (R: mem -> Prop);
+  requires t m := R m;
+  ensures t' m' res := t' = t /\
+                       <{ * cbt map.empty res
+                          * R }> m' #**/                                   /**.
+Derive cbt_init SuchThat (fun_correct! cbt_init) As cbt_init_ok.                .**/
+{                                                                          /**. .**/
+  return NULL;                                                             /**. .**/
+}                                                                          /**.
+unfold cbt. exists (map.empty). exists m. step. apply map.split_empty_l.
+step. step. right. unfold emp. tauto. tauto.
+Qed.
 
-#[local] Hint Extern 1 (cannot_purify (bst' _ _ _))
+
+#[local] Hint Extern 1 (cannot_purify (cbt' _ _ _))
       => constructor : suppressed_warnings.
-#[local] Hint Extern 1 (cannot_purify (bst _ _))
+#[local] Hint Extern 1 (cannot_purify (cbt _ _))
+      => constructor : suppressed_warnings.
+#[local] Hint Extern 1 (cannot_purify (nncbt _ _))
       => constructor : suppressed_warnings.
 #[local] Hint Extern 1 (cannot_purify (freeable _ _))
       => constructor : suppressed_warnings.
-
-#[local] Hint Unfold bst : heapletwise_always_unfold.
-
-Lemma invert_bst'_null{sk s p m}:
-    p = /[0] ->
-    m |= bst' sk s p ->
-    sk = Leaf /\
-    m |= emp (forall x, ~ s x).
-Proof.
-  unfold with_mem. intros. subst. destruct sk; simpl in *.
-  - unfold emp in *. intuition auto.
-  - repeat heapletwise_step. exfalso. apply H1. reflexivity.
-Qed.
-
-Lemma invert_bst'_nonnull{sk s p m}:
-    p <> /[0] ->
-    m |= bst' sk s p ->
-    exists skL skR pL v pR,
-      sk = Node skL skR /\
-      s v /\
-      <{ * freeable 12 p
-         * <{ + uintptr pL
-              + uint 32 v
-              + uintptr pR }> p
-         * bst' skL (fun x => s x /\ x < v) pL
-         * bst' skR (fun x => s x /\ v < x) pR }> m.
-Proof.
-  intros.
-  destruct sk; simpl in *|-.
-  { exfalso. unfold with_mem, emp in *. intuition idtac. }
-  repeat heapletwise_step.
-  do 5 eexists. split. 1: reflexivity.
-  split. 1: eassumption.
-  repeat heapletwise_step.
-Qed.
-
-  (* TODO use and move or delete *)
-  Lemma after_if_skip' b fs (PThen PElse Post: trace -> mem -> locals -> Prop):
-    bool_expr_branches b (forall t m l, PThen t m l -> Post t m l)
-                         (forall t m l, PElse t m l -> Post t m l) True ->
-    @after_if _ _ _ _ _ _ fs b PThen PElse cmd.skip Post.
-  Proof.
-    intros.
-    unfold after_if.
-    intros ? ? ? [? ? ?]. subst x.
-    eapply wp_skip.
-    apply proj1 in H.
-    destruct b; eauto.
-  Qed.
-
-Ltac step_hook ::=
-  match goal with
-  | |- _ => progress cbn [bst']
-  | sk: tree_skeleton |- _ => progress subst sk
-  | H: _ |= bst' _ _ ?p, E: ?p = /[0] |- _ =>
-      assert_fails (has_evar H); eapply (invert_bst'_null E) in H
-  | H: _ |= bst' _ _ ?p, N: ?p <> /[0] |- _ =>
-      assert_fails (has_evar H); eapply (invert_bst'_nonnull N) in H
-  | s: set Z, H: forall x: Z, ~ _ |- _ =>
-      lazymatch goal with
-      | |- context[s ?v] =>
-          lazymatch type of H with
-          | context[s] => unique pose proof (H v)
-          end
-      end
-  | |- ?A \/ ?B =>
-      tryif (assert_succeeds (assert (~ A) by (zify_goal; xlia zchecker)))
-      then right else
-      tryif (assert_succeeds (assert (~ B) by (zify_goal; xlia zchecker)))
-      then left else fail
-  | H1: ?x <= ?y, H2: ?y <= ?x, C: ?s ?x |- ?s ?y =>
-      (replace y with x by xlia zchecker); exact C
-  | |- _ => solve [auto 3]
-  end.
-
-(* TODO move *)
-Local Hint Extern 1 (cannot_purify (freeable _ _))
-      => constructor : suppressed_warnings.
-Local Hint Extern 1 (PredicateSize_not_found (freeable _))
-      => constructor : suppressed_warnings.
-Local Hint Extern 1 (PredicateSize_not_found allocator_failed_below)
-      => constructor : suppressed_warnings.
-Local Hint Extern 1 (PredicateSize_not_found (@allocator _ _))
-      => constructor : suppressed_warnings.
-Local Hint Extern 1 (cannot_purify allocator)
-      => constructor : suppressed_warnings.
-Local Hint Extern 1 (cannot_purify (if _ then _ else _))
+#[local] Hint Extern 1 (cannot_purify (or1 _ _))
       => constructor : suppressed_warnings.
 
-#[export] Instance spec_of_bst_init: fnspec :=                              .**/
+#[local] Hint Unfold cbt : heapletwise_always_unfold.
 
-uintptr_t bst_init( ) /**#
+#[export] Instance spec_of_dummy: fnspec := .**/
+uintptr_t dummy( ) /**#
   ghost_args := (R: mem -> Prop);
-  requires t m := <{ * allocator
+  requires t m := True;
+                  ensures t' m' res := True #**/ /**. About spec_of_dummy.
+
+Check .**/ void dummy( ) /**#
+  ghost_args := (R: mem -> Prop);
+  requires t m := True;
+                  ensures t' m' := True #**/ /**.
+
+Check spec_of_dummy : Semantics.env -> Prop.
+Print spec_of_dummy.
+
+#[export] Instance spec_of_cbt_best_leaf: fnspec :=                             .**/
+
+uintptr_t cbt_best_leaf(uintptr_t tp, uintptr_t k) /**#
+  ghost_args := (c: word_map) (R: mem -> Prop);
+  requires t m := <{ * nncbt c tp
                      * R }> m;
-  ensures t' m' res := t' = t /\
-                       <{ * (if \[res] =? 0 then
-                               allocator_failed_below 4
-                             else
-                               <{ * allocator
-                                  * bst (fun _ => False) res }>)
-                          * R }> m' #**/                                   /**.
-Derive bst_init SuchThat (fun_correct! bst_init) As bst_init_ok.                .**/
-{                                                                          /**. .**/
-  uintptr_t res = malloc(4);                                               /**. .**/
-  if (res == NULL) /* split */ {                                           /**. .**/
-    return NULL;                                                           /**. .**/
-  }                                                                        /**.
-    replace (\[/[0]] =? 0) with true by steps.
-    replace (0 =? 0) with true in * by steps.
-    steps.
-                                                                                .**/
-  else {                                                                   /**.
-    replace (\[res] =? 0) with false in * by steps.
-    let h := constr:(#(@sep)) in unfold with_mem, anyval in h.
-    step. step. step.
-    match goal with
-    | h: _ |- _ => change (with_mem m0 (array (uint 8) 4 v res)) in h
-    end.
-                                                                                .**/
-    store(res, NULL);                                                      /**. .**/
-    return res;                                                            /**. .**/
-  }                                                                        /**.
-    replace (\[res] =? 0) with false by steps.
-    steps.
-    instantiate (2 := Leaf). clear Error. unfold find_hyp_for_range. cbn [bst'].
-    steps.
-                                                                                .**/
-}                                                                          /**.
-Qed.
-
-#[export] Instance spec_of_bst_add: fnspec :=                              .**/
-
-uintptr_t bst_add(uintptr_t p, uintptr_t v) /**#
-  ghost_args := s (R: mem -> Prop);
-  requires t m := <{ * allocator
-                     * bst s p
-                     * R }> m;
-  ensures t' m' q := t' = t /\
-                     (if \[q] =? 0 then
-                        <{ * allocator_cannot_allocate 12
-                           * bst s p
-                           * R }> m'
-                      else
-                        <{ * allocator
-                           * bst (fun x => x = \[v] \/ s x) q
-                           * R }> m') #**/                                 /**.
-Derive bst_add SuchThat (fun_correct! bst_add) As bst_add_ok.                   .**/
-{                                                                          /**. .**/
-  uintptr_t a = load(p);                                                   /**.
-  (* invariant: *p = a *)                                                       .**/
-  uintptr_t found = 0;                                                     /**.
-
-  prove (found = /[1] -> s \[v]).
-  delete #(found = /[0]).
-  move sk after a.
-  move p after a.
-  loop invariant above a.
-  unfold ready.
-  lazymatch goal with
-  | |- exec ?fs ?body ?t ?m ?l ?P =>
-      lazymatch eval pattern R in P with
-      | ?f R =>
-          change (exec fs body t m l ((fun (g: set Z * (mem -> Prop)) (_: tree_skeleton) =>
-            let (_, F) := g in f F) (s, R) sk))
-      end
-  end.
-  let e := constr:(live_expr:(a != NULL && !found)) in
-  eapply (wp_while_tailrec_use_functionpost _ _ e).
-  { eauto with wf_of_type. }
-  { (* Ltac log_packaged_context P ::= idtac P. *)
-    package_heapletwise_context. }
-  start_loop_body.
-  steps.
-                                                                                .**/
-    uintptr_t x = load32(a + 4);                                           /**. .**/
-    if (x == v) {                                                          /**. .**/
-      found = 1;                                                           /**. .**/
-    } else {                                                               /**. .**/
-      if (v < x) {                                                         /**. .**/
-        p = a;                                                             /**. .**/
-        a = load(p);                                                       /**. .**/
-      } else {                                                             /**. .**/
-        p = a + 8;                                                         /**. .**/
-        a = load(p);                                                       /**. .**/
-      }                                                                    /**.
-      (* TODO can we pull this out of the branches?
-        a = load(p);                         *)                                 .**/
-    }                                                                      /**. .**/
-  }                                                                        /**.
-
+  ensures t' m' res := t' = t /\ ex1 (fun k' => ex1 (fun v' =>
+                  let leaf := cbt' Leaf (full_prefix k') (map.singleton k' v') res in
+                        <{ * leaf
+                           * wand leaf (nncbt c tp)
+                           * emp (k <> k' <-> map.get c k = None)}> )) m' #**/     /**.
+Derive cbt_best_leaf SuchThat (fun_correct! cbt_best_leaf) As cbt_best_leaf_ok.  .**/
+{                                                                            /**. .**/
+  uintptr_t p = tp;                                                            /**.
+  loop invariant above Def0. .**/
+  while (load32(p) != 0) /* decreases (1) */ {                        /**.
+  (* the termination measure should be the tree skeleton. How do we get
+     the skeleton out of p? *)
+  (* -> ?apply the while rule manually? *)
 Abort.
 
-#[export] Instance spec_of_bst_contains: fnspec :=                              .**/
-
-uintptr_t bst_contains(uintptr_t p, uintptr_t v) /**#
-  ghost_args := s (R: mem -> Prop);
-  requires t m := <{ * bst s p
+#[export] Instance spec_of_cbt_lookup: fnspec :=                                .**/
+(* parameter "d" for "default" *)
+uintptr_t cbt_lookup(uintptr_t tp, uintptr_t k, uintptr_t d) /**#
+  ghost_args := (c: word_map) (R: mem -> Prop);
+  requires t m := <{ * cbt c tp
                      * R }> m;
-  ensures t' m' b := t' = t /\
-                     (\[b] = 1 /\ s \[v] \/ \[b] = 0 /\ ~ s \[v]) /\
-                     <{ * bst s p
-                        * R }> m' #**/                                     /**.
-Derive bst_contains SuchThat (fun_correct! bst_contains) As bst_contains_ok.    .**/
-{                                                                          /**. .**/
-  uintptr_t res = 0;                                                       /**. .**/
-  uintptr_t a = load(p);                                                   /**.
+  ensures t' m' res := t' = t
+           /\ <{ * emp (match map.get c k with | Some v => v | None => d end = res)
+                 * cbt c tp
+                 * R }> m'         #**/                                     /**.
+Derive cbt_lookup SuchThat (fun_correct! cbt_lookup) As cbt_lookup_ok.           .**/
+{                                                                           /**. .**/
+  if (tp == NULL) /* split */ {                                             /**. .**/
+    return d;                                                               /**. .**/
+  }                                                                         /*?.
+  step. step. step. step. step.  destruct H0. destruct H0. destruct H0.
+  destruct x; simpl in H0. step. step. step. step. step. step. step. step.
+  step. step. step. step. step. step. step. step. step. step. step. step.
+  step. step. step. step. step. step. step. step. step. step. step. step.
+  step. step. step. step. step. step. subst c. rewrite map.get_empty. step.
+  subst tp. steps.                                                               .**/
+  else {                                                                    /**.
+  Abort.
 
-  let h := constr:(#bst') in loop pre above h.
-  (* TODO this step is needed because `m2 |= uintptr a p` will get pulled into
-     the loop pre/post even though it could remain outside (because we currently
-     mention the whole memory in the loop). Better: Use/integrate frame rule in
-     loop rule so that unneeded mem hyps can stay outside *)
-  let h := constr:(#(uintptr a p)) in remember a as root in h.
+#[export] Instance spec_of_cbt_insert: fnspec :=                                  .**/
 
-  unfold ready.
-  let cond := constr:(live_expr:(!res && a != 0)) in
-  let measure0 := constr:(sk) in
-  eapply (wp_while_tailrec_with_done_flag measure0 (s, a, R) cond).
-  1: eauto with wf_of_type.
-  { collect_heaplets_into_one_sepclause.
-    package_context. }
-  { start_loop_body.
-    steps.
-    { (* loop condition false implies post (which could be constructed here from
-         the context, hopefully) *)
-      instantiate (1 := fun '(s, olda, F, sk, ti, mi, li) =>
-                        exists newa res,
-                        li = map.of_list [|("a", newa); ("p", p); ("res", res); ("v", v)|] /\
-                          <{ * uintptr a p
-                             * freeable 4 p
-                             * bst' sk s olda
-                             * F }> mi /\
-                        (\[res] = 1 /\ s \[v] \/ \[res] = 0 /\ ~ s \[v]) /\
-                        ti = t).
-      cbv beta iota.
-      cbn [bst']. (* <-- TODO step_hook invoked too late *)
-      step. step. step. step.
-      steps.
-    }
-    (* loop body: *)
-                                                                                .**/
-    uintptr_t here = load32(a+4);                                          /**. .**/
-    if (v < here) /* split */ {                                            /**. .**/
-      a = load(a);                                                         /**. .**/
-    }                                                                      /**. .**/
-    else {                                                                 /**. .**/
-      if (here < v) /* split */ {                                          /**. .**/
-        a = load(a+8);                                                     /**. .**/
-      }                                                                    /**. .**/
-      else {                                                               /**. .**/
-        res = 1;                                                           /**. .**/
-      }                                                                    /**. .**/
-    }                                                                      /**. .**/
-  }                                                                        /**.
-  }
-  (* after loop *)
-  subst a. clear res Def0.
-  clear_until_LoopInvOrPreOrPost_marker.
-  steps.
-  subst l.
-                                                                                .**/
-  return res;                                                              /**. .**/
-}                                                                          /**.
-Qed.
-
-(* note: inability to break out of loop is cumbersome, because it complicates pre:
-   it has to incorporate almost all of post for the res=true case,
-   and even if we break, we still have to decrease the termination measure *)
-
-*)
+uintptr_t cbt_insert(uintptr_t tp, uintptr_t k, uintptr_t v) /**#
+  ghost_args := (c c': word_map) (R: mem -> Prop);
+  requires t m := <{ * cbt c tp
+                     * R }> m;
+  ensures t' m' res := t' = t
+           /\ <{ * emp (map.put c k v = c') (* should this really be equality? *)
+                 * cbt c' res
+                 * R }> m'        #**/                                      /**.
+Derive cbt_insert SuchThat (fun_correct! cbt_insert) As cbt_insert_ok.
+(* TODO: implement & prove *)
+Abort.
 
 End LiveVerif. Comments .**/ //.
